isConstantTime proof for instruction

src/arch/x64/X64.Leakage_i.fst
@@ -54,6 +54,21 @@ let rec operands_do_not_use_secrets ops ts = match ops with
   | [] -> true
   | hd :: tl -> operand_does_not_use_secrets hd ts && (operands_do_not_use_secrets tl ts)
 
+val lemma_operands_imply_op: (ts:taintState) -> (ops:list operand{Cons? ops}) -> Lemma
+(requires (operands_do_not_use_secrets ops ts))
+(ensures (operand_does_not_use_secrets (List.Tot.Base.hd ops) ts))
+
+let lemma_operands_imply_op ts ops = match ops with
+| hd :: tl -> ()
+
+val lemma_operand_obs_list: (ts:taintState) -> (ops:list operand) -> (s1:traceState) -> (s2:traceState) -> Lemma 
+(requires (operands_do_not_use_secrets ops ts /\ publicValuesAreSame ts s1 s2))
+(ensures  (operand_obs_list s1 ops) = (operand_obs_list s2 ops))
+
+let rec lemma_operand_obs_list ts ops s1 s2 = match ops with
+  | [] -> ()
+  | hd :: tl -> assert (operand_does_not_use_secrets hd ts); assert_by_tactic (operand_obs s1 hd = operand_obs s2 hd) (apply_lemma (quote (lemma_operand_obs ts))); lemma_operand_obs_list ts tl s1 s2
+
 let rec sources_taint srcs ts taint = match srcs with
   | [] -> taint
   | hd :: tl -> merge_taint (operand_taint hd ts) (sources_taint tl ts taint)
@@ -67,15 +82,15 @@ val check_if_ins_consumes_fixed_time: (ins:tainted_ins) -> (ts:taintState) -> (r
 let check_if_ins_consumes_fixed_time ins ts =
   let i, dsts, srcs = ins.ids in
   let ftSrcs = operands_do_not_use_secrets srcs ts in
-  let ftDsts = operands_do_not_use_secrets (List.Tot.Base.map dst_to_op dsts) ts in
+  let dsts2 = List.Tot.Base.map dst_to_op dsts in
+  let ftDsts = operands_do_not_use_secrets dsts2 ts in
   let fixedTime = ftSrcs && ftDsts in
 
-  assert_by_tactic (forall dst s1 s2. (operand_does_not_use_secrets dst ts /\ publicValuesAreSame ts s1 s2)  ==>
-    (operand_obs s1 dst) = (operand_obs s2 dst)) (dst <-- forall_intro; s1 <-- forall_intro; s2 <-- forall_intro; h <-- implies_intro; apply_lemma (quote (lemma_operand_obs ts)));
+  assert_by_tactic (forall s1 s2. (operands_do_not_use_secrets dsts2 ts /\ publicValuesAreSame ts s1 s2) ==>
+    (operand_obs_list s1 dsts2) = (operand_obs_list s2 dsts2)) (s1 <-- forall_intro; s2 <-- forall_intro; h <-- implies_intro; apply_lemma (quote (lemma_operand_obs_list ts dsts2))); 
 
-  assert (forall s1 s2. (operands_do_not_use_secrets dsts ts /\ publicValuesAreSame ts s1 s2) ==>
-    (operand_obs_list s1 dsts) = (operand_obs_list s2 dsts));
-(*  assert (fixedTime ==> (isConstantTime (Ins ins) ts)); *)
+  assert_by_tactic (forall s1 s2. (operands_do_not_use_secrets srcs ts /\ publicValuesAreSame ts s1 s2) ==> (operand_obs_list s1 srcs) = (operand_obs_list s2 srcs)) (s1 <-- forall_intro; s2 <-- forall_intro; h <-- implies_intro; apply_lemma (quote (lemma_operand_obs_list ts srcs)));
+  assert (fixedTime ==> (isConstantTime (Ins ins) ts));
   let taint = sources_taint srcs ts ins.t in
   let ts' = set_taints dsts ts taint in
   (* TODO : Probably check on dsts for fixedTime *)
